

Series

Sunday, 14 December 2025 9:22 pm

SERIES:

The sum of the terms of a sequence forms a series. If a_1, a_2, a_3, \dots represent a sequence of numbers, then the corresponding series is

$$a_1 + a_2 + a_3 + \dots = \sum_{k=1}^{\infty} a_k$$

SUMMATION NOTATION:

The capital Greek letter sigma Σ is used to write a sum in a short hand notation. where k varies from 1 to n represents the sum given in expanded form by

$$= a_1 + a_2 + a_3 + \dots + a_n$$

More generally if m and n are integers and $m \leq n$, then the summation from k equal m to n of a_k is

$$\sum_{k=m}^n a_k = a_m + a_{m+1} + a_{m+2} + \dots + a_n$$

Here **k** is called the index of the summation; **m** the lower limit of the summation and **n** the upper limit of the summation.

COMPUTING SUMMATIONS:

Let $a_0 = 2, a_1 = 3, a_2 = -2, a_3 = 1$ and $a_4 = 0$. Compute each of the summations:

$$(a) \quad \sum_{i=0}^4 a_i \qquad (b) \quad \sum_{j=0}^2 a_{2j} \qquad (c) \quad \sum_{k=1}^1 a_k$$

SOLUTION:

$$(a) \quad \sum_{i=0}^4 a_i = a_0 + a_1 + a_2 + a_3 + a_4 \\ = 2 + 3 + (-2) + 1 + 0 = 4$$

$$(b) \quad \sum_{j=0}^2 a_{2j} = a_0 + a_2 + a_4 \\ = 2 + (-2) + 0 = 0$$

$$(c) \quad \sum_{k=1}^1 a_k = a_1 \\ = 3$$

EXERCISE:

Compute the summations

$$1. \quad \sum_{i=1}^3 (2i-1) = [2(1)-1] + [2(2)-1] + [2(3)-1] \\ = 1 + 3 + 5 \\ = 9$$

$$\begin{aligned}
 2. \quad \sum_{k=-1}^1 (k^3 + 2) &= [(-1)^3 + 2] + [(0)^3 + 2] + [(1)^3 + 2] \\
 &= [-1 + 2] + [0 + 2] + [1 + 2] \\
 &= 1 + 2 + 3 \\
 &= 6
 \end{aligned}$$

SUMMATION NOTATION TO EXPANDED FORM:

Write the summation $\sum_{i=0}^n \frac{(-1)^i}{i+1}$ to expanded form.

SOLUTION:

$$\begin{aligned}
 \sum_{i=0}^n \frac{(-1)^i}{i+1} &= \frac{(-1)^0}{0+1} + \frac{(-1)^1}{1+1} + \frac{(-1)^2}{2+1} + \frac{(-1)^3}{3+1} + \cdots + \frac{(-1)^n}{n+1} \\
 &= \frac{1}{1} + \frac{(-1)}{2} + \frac{1}{3} + \frac{(-1)}{4} + \cdots + \frac{(-1)^n}{n+1} \\
 &= 1 - \frac{1}{2} + \frac{1}{3} - \frac{1}{4} + \cdots + \frac{(-1)^n}{n+1}
 \end{aligned}$$

EXPANDED FORM TO SUMMATION NOTATION:

Write the following using summation notation:

$$1. \quad \frac{1}{n} + \frac{2}{n+1} + \frac{3}{n+2} + \cdots + \frac{n+1}{2n}$$

SOLUTION:

We find the kth term of the series.

The numerators forms an arithmetic sequence 1, 2, 3, ..., n+1, in which

$$a = \text{first term} = 1$$

& $d = \text{common difference} = 1$

$$a_k = a + (k - 1)d$$

$$= 1 + (k - 1)(1) = 1 + k - 1 = k$$

Similarly, the denominators forms an arithmetic sequence

n, n+1, n+2, ..., 2n, in which

$$a = \text{first term} = n$$

$$d = \text{common difference} = 1$$

$$\begin{aligned}
 \therefore a_k &= a + (k - 1)d \\
 &= n + (k - 1)(1) \\
 &= k + n - 1
 \end{aligned}$$

Hence the kth term of the series is

$$\frac{k}{(n-1) + k}$$

And the expression for the series is given by

$$\begin{aligned}\therefore \frac{1}{n} + \frac{2}{n+1} + \frac{3}{n+2} + \cdots + \frac{n+1}{2n} &= \sum_{k=1}^{n+1} \frac{k}{(n-1)+k} \\ &= \sum_{k=0}^n \frac{k+1}{n+k}\end{aligned}$$

TRANSFORMING A SUM BY A CHANGE OF VARIABLE:

Consider $\sum_{k=1}^3 k^2 = 1^2 + 2^2 + 3^2$

and $\sum_{i=1}^3 i^2 = 1^2 + 2^2 + 3^2$

Hence $\sum_{k=1}^3 k^2 = \sum_{i=1}^3 i^2$

The index of a summation can be replaced by any other symbol. The index of a summation is therefore called a dummy variable.

EXERCISE:

Consider $\sum_{k=1}^{n+1} \frac{k}{(n-1)+k}$

Substituting $k = j + 1$ so that $j = k - 1$

When $k = 1, j = k - 1 = 1 - 1 = 0$

When $k = n + 1, j = k - 1 = (n + 1) - 1 = n$

Hence

$$\begin{aligned}\sum_{k=1}^{n+1} \frac{k}{(n-1)+k} &= \sum_{j=0}^n \frac{j+1}{(n-1)+(j+1)} \\ &= \sum_{j=0}^n \frac{j+1}{n+j} = \sum_{k=0}^n \frac{k+1}{n+k} \quad (\text{changing variable})\end{aligned}$$

Transform by making the change of variable $j = i - 1$, in the summation

$$\sum_{i=1}^{n-1} \frac{i}{(n-i)^2} \quad **$$

PROPERTIES OF SUMMATIONS:

1. $\sum_{k=m}^n (a_k + b_k) = \sum_{k=m}^n a_k + \sum_{k=m}^n b_k; \quad a_k, b_k \in R$
2. $\sum_{k=m}^n c a_k = c \sum_{k=m}^n a_k \quad c \in R$
3. $\sum_{k=a-i}^{b-i} (k+i) = \sum_{k=a}^b k \quad i \in N$

$$4. \sum_{k=a+i}^{b+i} (k-i) = \sum_{k=a}^b k \quad i \in \mathbb{N}$$

$$5. \sum_{k=1}^n c = c + c + \dots + c = nc$$

EXERCISE:

Express the following summation more simply:

SOLUTION:

$$\begin{aligned} & 3 \sum_{k=1}^n (2k-3) + \sum_{k=1}^n (4-5k) \\ & 3 \sum_{k=1}^n (2k-3) + \sum_{k=1}^n (4-5k) \\ & = 3 \sum_{k=1}^n 3(2k-3) + \sum_{k=1}^n (4-5k) \\ & = \sum_{k=1}^n [3(2k-3) + (4-5k)] \\ & = \sum_{k=1}^n (k-5) \\ & = \sum_{k=1}^n k - \sum_{k=1}^n 5 \\ & = \sum_{k=1}^n k - 5n \end{aligned}$$

ARITHMETIC SERIES:

The sum of the terms of an arithmetic sequence forms an arithmetic series (A.S). For example

$$1 + 3 + 5 + 7 + \dots$$

is an arithmetic series of positive odd integers.

In general, if a is the first term and d the common difference of an arithmetic series, then the series is given as: $a + (a+d) + (a+2d) + \dots$

SUM OF n TERMS OF AN ARITHMETIC SERIES:

Let a be the first term and d be the common difference of an arithmetic series. Then its n th term is:

$$a_n = a + (n-1)d; \quad n \geq 1$$

If S_n denotes the sum of first n terms of the A.S, then

$$\begin{aligned} S_n &= a + (a+d) + (a+2d) + \dots + [a + (n-1)d] \\ &= a + (a+d) + (a+2d) + \dots + a_n \\ &= a + (a+d) + (a+2d) + \dots + (a_n - d) + a_n \dots \dots \dots (1) \end{aligned}$$

where $a_n = a + (n-1)d$

Rewriting the terms in the series in reverse order,

$$S_n = a_n + (a_n - d) + (a_n - 2d) + \dots + (a + d) + a \dots \dots \dots (2)$$

Adding (1) and (2) term by term, gives

$$\begin{aligned}
 2 S_n &= (a + a_n) + (a + a_n) + (a + a_n) + \dots + (a + a_n) \quad (n \text{ terms}) \\
 2 S_n &= n (a + a_n) \\
 \Rightarrow S_n &= n(a + a_n)/2 \\
 S_n &= n(a + l)/2 \dots\dots\dots(3) \\
 \text{Where } l &= a_n = a + (n - 1)d
 \end{aligned}$$

Where

Therefore

$$\begin{aligned}
 S_n &= n/2 [a + a + (n - 1) d] \\
 S_n &= n/2 [2 a + (n - 1) d] \dots\dots\dots(4)
 \end{aligned}$$

EXERCISE:

Find the sum of first n natural numbers.

SOLUTION:

Let $S_n = 1 + 2 + 3 + \dots + n$

Clearly the right hand side forms an arithmetic series with

$$a = 1, \quad d = 2 - 1 = 1 \quad \text{and} \quad n = n$$

$$\begin{aligned}
 \therefore S_n &= \frac{n}{2} [2a + (n-1)d] \\
 &= \frac{n}{2} [2(1) + (n-1)(1)] \\
 &= \frac{n}{2} [2 + n - 1] \\
 &= \frac{n(n+1)}{2}
 \end{aligned}$$

EXERCISE:

Find the sum of all two digit positive integers which are neither divisible by 5 nor by 2.

SOLUTION:

The series to be summed is:

$$11 + 13 + 17 + 19 + 21 + 23 + 27 + 29 + \dots + 91 + 93 + 97 + 99$$

which is not an arithmetic series.

If we make group of four terms we get

$$(11 + 13 + 17 + 19) + (21 + 23 + 27 + 29) + (31 + 33 + 37 + 39) + \dots + (91 + 93 + 97 + 99) = 60 + 100 + 140 + \dots + 380$$

which now forms an arithmetic series in which

$$a = 60; \quad d = 100 - 60 = 40 \quad \text{and} \quad l = a_n = 380$$

To find n, we use the formula

$$\begin{aligned}
 a_n &= a + (n - 1) d \\
 \Rightarrow 380 &= 60 + (n - 1) (40) \\
 \Rightarrow 380 - 60 &= (n - 1) (40) \\
 \Rightarrow 320 &= (n - 1) (40)
 \end{aligned}$$

$$\frac{320}{40} = n - 1$$

$$\begin{aligned} 8 &= n - 1 \\ \Rightarrow n &= 9 \end{aligned}$$

Now

$$\begin{aligned} S_n &= \frac{n}{2}(a + l) \\ \therefore S_9 &= \frac{9}{2}(60 + 380) = 1980 \end{aligned}$$

GEOMETRIC SERIES:

The sum of the terms of a geometric sequence forms a geometric series (G.S.). For example

$$1 + 2 + 4 + 8 + 16 + \dots$$

is geometric series.

In general, if **a** is the first term and **r** the common ratio of a geometric series, then the series is given as: $a + ar + ar^2 + ar^3 + \dots$

SUM OF n TERMS OF A GEOMETRIC SERIES:

Let **a** be the first term and **r** be the common ratio of a geometric series. Then its nth term is:

$$a_n = ar^{n-1}; \quad n \geq 1$$

If S_n denotes the sum of first n terms of the G.S. then

$$S_n = a + ar + ar^2 + ar^3 + \dots + ar^{n-2} + ar^{n-1} \dots \dots \dots (1)$$

Multiplying both sides by r we get.

$$r S_n = ar + ar^2 + ar^3 + \dots + ar^{n-1} + ar^n \dots \dots \dots (2)$$

Subtracting (2) from (1) we get

$$S_n - rS_n = a - ar^n$$

$$\Rightarrow (1 - r) S_n = a (1 - r^n)$$

$$\Rightarrow S_n = \frac{a(1-r^n)}{1-r} \quad (r \neq 1)$$

EXERCISE:

Find the sum of the geometric series

$$6 - 2 + \frac{2}{3} - \frac{2}{9} + \dots + \text{to 10 terms}$$

SOLUTION:

In the given geometric series

$$a = 6, \quad r = \frac{-2}{6} = -\frac{1}{3} \quad \text{and } n = 10$$

$$\begin{aligned} \therefore S_n &= \frac{a(1-r^n)}{1-r} \\ S_{10} &= \frac{6 \left(1 - \left(-\frac{1}{3} \right)^{10} \right)}{1 - \left(-\frac{1}{3} \right)} = \frac{6 \left(1 + \frac{1}{3^{10}} \right)}{\left(\frac{4}{3} \right)} \\ &= \frac{9 \left(1 + \frac{1}{3^{10}} \right)}{2} \end{aligned}$$

INFINITE GEOMETRIC SERIES:

Consider the infinite geometric series

$$a + ar + ar^2 + \dots + ar^{n-1} + \dots$$

then

$$S_n = a + ar + ar^2 + \dots + ar^{n-1} = \frac{a(1-r^n)}{1-r} \quad (r \neq 1)$$

If $S_n \rightarrow S$ as $n \rightarrow \infty$, then the series is convergent and S is its sum.

If $|r| < 1$, then $r^n \rightarrow 0$ as $n \rightarrow \infty$

$$\begin{aligned} \therefore S &= \lim_{n \rightarrow \infty} S_n = \lim_{n \rightarrow \infty} \frac{a(1-r^n)}{1-r} \\ &= \frac{a}{1-r} \end{aligned}$$

If S_n increases indefinitely as n becomes very large then the series is said to be divergent.

EXERCISE:

Find the sum of the infinite geometric series:

$$\frac{9}{4} + \frac{3}{2} + 1 + \frac{2}{3} + \dots$$

SOLUTION:

Here we have

$$a = \frac{9}{4}, \quad r = \frac{3/2}{9/4} = \frac{2}{3}$$

Note that $|r| < 1$ So we can use the above formula.

$$\begin{aligned} \therefore S &= \frac{a}{1-r} \\ &= \frac{9/4}{1-2/3} \\ &= \frac{9/4}{1/3} = \frac{9}{4} \times \frac{3}{1} = \frac{27}{4} \end{aligned}$$

EXERCISE:

Find a common fraction for the recurring decimal 0.81

SOLUTION:

$$\begin{aligned} 0.81 &= 0.8181818181 \dots \\ &= 0.81 + 0.0081 + 0.000081 + \dots \end{aligned}$$

which is an infinite geometric series with

$$a = 0.81, \quad r = \frac{0.0081}{0.81} = 0.01$$

$$\begin{aligned} \therefore \text{Sum} &= \frac{a}{1-r} \\ &= \frac{0.81}{1-0.01} = \frac{0.81}{0.99} \\ &= \frac{81}{99} = \frac{9}{11} \end{aligned}$$

IMPORTANT SUMS:

1. $1 + 2 + 3 + \dots + n = \sum_{k=1}^n k = \frac{n(n+1)}{2}$
2. $1^2 + 2^2 + 3^2 + \dots + n^2 = \sum_{k=1}^n k^2 = \frac{n(n+1)(2n+1)}{6}$
3. $1^3 + 2^3 + 3^3 + \dots + n^3 = \sum_{k=1}^n k^3 = \frac{n^2(n+1)}{4} = \left[\frac{n(n+1)}{2} \right]^2$

